ocaml/src/QcertOut.ml
@@ -41,6 +41,7 @@ let output_query pconf q =
   | QcertCompiler.Q_cldmr q -> pretty_query pconf pretty_cldmr q
   | QcertCompiler.Q_dnnrc q -> pretty_query pconf pretty_dnnrc q
   | QcertCompiler.Q_dnnrc_typed q -> pretty_query pconf pretty_dnnrc_typed q
+  | QcertCompiler.Q_js_ast q -> pretty_query pconf pretty_js_ast q
   | QcertCompiler.Q_javascript q -> pretty_query pconf pretty_javascript q
   | QcertCompiler.Q_java q -> pretty_query pconf pretty_java q
   | QcertCompiler.Q_spark_rdd q -> pretty_query pconf pretty_spark_rdd q
