coq/Compiler/Driver/CompEval.v
@@ -43,6 +43,7 @@ Section CompEval.
   Require Import tDNNRCRuntime.
   Require Import CAMPRuntime.
   (** Target languages *)
+  Require Import JsAst.JsSyntax.
   Require Import JavaScriptRuntime.
   Require Import JavaRuntime.
   Require Import SparkRDDRuntime.
@@ -181,6 +182,7 @@ Section CompEval.
       | Q_cldmr q => lift_output (eval_cldmr q (lift_input ev_in))
       | Q_dnnrc q => lift_output (eval_dnnrc q ev_in) (* XXX Does not localize, keeps distributed information XXX *)
       | Q_dnnrc_typed q => lift_output (eval_dnnrc_typed q ev_in) (* XXX Does not localize, keeps distributed information XXX *)
+      | Q_js_ast _ => Ev_out_unsupported ("No evaluation support for "++(name_of_language (language_of_query q))) (* XXX TODO XXX *)
       | Q_javascript _ => Ev_out_unsupported ("No evaluation support for "++(name_of_language (language_of_query q)))
       | Q_java _ => Ev_out_unsupported ("No evaluation support for "++(name_of_language (language_of_query q)))
       | Q_spark_rdd _ => Ev_out_unsupported ("No evaluation support for "++(name_of_language (language_of_query q)))
@@ -210,6 +212,7 @@ Section CompEval.
       | Q_cldmr _ => Ev_out_unsupported ("No debug evaluation support for "++(name_of_language (language_of_query q)))
       | Q_dnnrc _ => Ev_out_unsupported ("No debug evaluation support for "++(name_of_language (language_of_query q)))
       | Q_dnnrc_typed _ => Ev_out_unsupported ("No debug evaluation support for "++(name_of_language (language_of_query q)))
+      | Q_js_ast _ => Ev_out_unsupported ("No debug evaluation support for "++(name_of_language (language_of_query q)))
       | Q_javascript _ => Ev_out_unsupported ("No debug evaluation support for "++(name_of_language (language_of_query q)))
       | Q_java _ => Ev_out_unsupported ("No debug evaluation support for "++(name_of_language (language_of_query q)))
       | Q_spark_rdd _ => Ev_out_unsupported ("No debug evaluation support for "++(name_of_language (language_of_query q)))
